Instances/Examples/Tier0Increment.lean
@@ -20,7 +20,8 @@ instance : Fintype ToyReg where
     cases r <;> simp
 
 def block : Block ToyReg :=
-  { stmts := [Stmt.put .r0 (.add64 (.get .r0) (.const 1))]
+  { stmts := [Stmt.put .r0 (.add64 (.get .r0) (.const 1)),
+              Stmt.put .r1 (.const 0)]
     ip_reg := .r1
     next := 0 }
 
